Port pan_globals fperm_decs_decls and new_main_name_correct

Flapjack/Test/CompilerParity.lean
@@ -41,6 +41,7 @@ import Flapjack.Test.PanGlobalsFunctionsFilterNilParity
 import Flapjack.Test.PanGlobalsFpermClusterParity
 import Flapjack.Test.PanGlobalsDecShapesClusterParity
 import Flapjack.Test.PanGlobalsFunctionPreservationParity
+import Flapjack.Test.PanGlobalsNameCorrectnessParity
 import Flapjack.Test.PanLangFunctionsParity
 import Flapjack.Test.CrepeDestConstParity
 import Flapjack.Test.CrepeDest2ExpParity
@@ -647,6 +648,7 @@ def main : IO Unit := do
     Flapjack.Test.PanGlobalsFpermClusterParity.runChecks,
     Flapjack.Test.PanGlobalsDecShapesClusterParity.runChecks,
     Flapjack.Test.PanGlobalsFunctionPreservationParity.runChecks,
+    Flapjack.Test.PanGlobalsNameCorrectnessParity.runChecks,
     Flapjack.Test.PanLangFunctionsParity.runChecks,
     Flapjack.Test.PanShapeValParity.runChecks,
     Flapjack.Test.LoopIsLoadParity.runChecks,
